first draft of state_rel for bvp-to-word compiler

compiler/closLangScript.sml
@@ -12,6 +12,7 @@ val _ = Datatype `
      | SetGlobal num (* assign a value to a global *)
      | AllocGlobal   (* make space for a new global *)
      | GlobalsPtr    (* get pointer to globals array *)
+   (* TODO: Add SetGlobalsPtr *)
      | Cons num      (* construct a Block with given tag *)
      | El            (* read Block field index *)
      | LengthBlock   (* get length of Block *)
