compiler/proofs/bvp_to_wordProofScript.sml
@@ -1,14 +1,126 @@
 open preamble bvlSemTheory bvpSemTheory bvpPropsTheory copying_gcTheory
-     int_bitwiseTheory;
+     int_bitwiseTheory bvp_to_wordPropsTheory finite_mapTheory
+     bvp_to_wordTheory;
 
 val _ = new_theory "bvp_to_wordProof";
 
 (* -------------------------------------------------------
     TODO:
-     - define state_rel
      - sketch compiler proof
+       - prove Return
+       - prove Seq
+       - prove Raise
+       - prove Assign Const
    ------------------------------------------------------- *)
 
+(* definition of state relation *)
 
+val isWord_def = Define `
+  (isWord (Word w) = T) /\ (isWord _ = F)`;
+
+val theWord_def = Define `
+  theWord (Word w) = w`;
+
+val code_rel_def = Define `
+  code_rel c s_code t_code <=>
+    !n arg_count prog.
+      (lookup n s_code = SOME (arg_count:num,prog)) ==>
+      ?k. (lookup n t_code = SOME (arg_count,FST (comp c n 1 prog),k))`
+
+val stack_rel_def = Define `
+  (stack_rel (Env env) (StackFrame vs NONE) <=>
+     !n. IS_SOME (lookup n env) <=>
+         IS_SOME (lookup (adjust_var n) (fromAList vs))) /\
+  (stack_rel (Exc env n) (StackFrame vs (SOME (x1,x2,x3))) <=>
+     stack_rel (Env env) (StackFrame vs NONE) /\ (x1 = n)) /\
+  (stack_rel _ _ <=> F)`
+
+val flat_def = Define `
+  (flat [] = []) /\
+  (flat (Env env::xs) = MAP SND (toAList env) ++ flat xs) /\
+  (flat (Exc env n::xs) = MAP SND (toAList env) ++ flat xs)`;
+
+val flat2_def = Define `
+  (flat2 (Env env::xs) (StackFrame vs _::ys) =
+     MAP (\(n,_). THE (ALOOKUP vs (adjust_var n))) (toAList env) ++ flat2 xs ys) /\
+  (flat2 (Exc env _::xs) (StackFrame vs _::ys) =
+     MAP (\(n,_). THE (ALOOKUP vs (adjust_var n))) (toAList env) ++ flat2 xs ys) /\
+  (flat2 _ _ = [])`;
+
+val state_rel_def = Define `
+  state_rel c l1 l2 (s:bvpSem$state) (t:'a wordSem$state) v1 w1 <=>
+    (* I/O, clock and handler are the same, GC is fixed, code is compiled *)
+    (t.io = s.io) /\
+    (t.clock = s.clock) /\
+    (t.handler = s.handler) /\
+    (t.gc_fun = word_gc_fun c) /\
+    code_rel c s.code t.code /\
+    (* the store contains everything except Handler *)
+    EVERY (\n. n IN FDOM t.store /\ isWord (t.store ' n))
+      [NextFree; LastFree; FreeCount; CurrHeap; OtherHeap; AllocSize; ProgStart] /\
+    EVERY (\n. n IN FDOM t.store) [Globals] /\
+    (* every local is represented in word lang *)
+    (lookup 0 t.locals = SOME (Loc l1 l2)) /\
+    (!n. IS_SOME (lookup n s.locals) ==>
+         IS_SOME (lookup (adjust_var n) t.locals)) /\
+    (* the stacks contain the same names, have same shape *)
+    EVERY2 stack_rel s.stack t.stack /\
+    (* there exists some GC-compatible abstraction *)
+    ?heap limit heap_addr_stack a sp.
+      (* the abstract heap is stored in memory *)
+      (word_heap (theWord (t.store ' CurrHeap)) heap c heap *
+       word_heap (theWord (t.store ' OtherHeap))
+         [Unused (limit-1)] c [Unused (limit-1)])
+           (fun2set (t.memory,t.mdomain)) /\
+      (* the abstract heap relates to the values of BVP *)
+      abs_ml_inv
+        (flat (Env v1 :: Env s.locals :: Env (insert 0 s.global LN) :: s.stack))
+        s.refs (heap_addr_stack,heap,F,a,sp) limit /\
+      s.space <= sp /\
+      (* word lang locals, globals and stack are correct *)
+      EVERY2 (\v w. word_addr c heap v = w) heap_addr_stack
+        (flat2 (Env v1 :: Env s.locals :: Env (insert 0 s.global LN) :: s.stack)
+               (StackFrame (toAList w1) NONE ::
+                StackFrame (toAList t.locals) NONE ::
+                StackFrame [(adjust_var 0, t.store ' Globals)] NONE ::
+                t.stack))`
+
+(* compiler proof *)
+
+val compile_correct = prove(
+  ``!(prog:bvp$prog) s c n l l1 l2 res s1 t.
+      (bvpSem$evaluate (prog,s) = (res,s1)) /\
+      res <> SOME (Rerr (Rabort Rtype_error)) /\
+      state_rel c l1 l2 s t LN LN ==>
+      ?t1 res1. (wordSem$evaluate (FST (comp c n l prog),t) = (res1,t1)) /\
+                (res1 <> SOME NotEnoughSpace ==>
+                 case res of
+                 | NONE => state_rel c l1 l2 s1 t1 LN LN /\ (res1 = NONE)
+                 | SOME (Rval v) =>
+                     ?w. state_rel c l1 l2 s1 t1 (insert 0 v LN)
+                            (insert (adjust_var 0) w LN) /\
+                         (res1 = SOME (Result w (Loc l1 l2)))
+                 | SOME (Rerr (Rraise v)) =>
+                     ?w. state_rel c l1 l2 s1 t1 (insert 0 v LN)
+                            (insert (adjust_var 0) w LN) /\
+                         (res1 = SOME (Exception w w))
+                 | SOME (Rerr (Rabort e)) => (res1 = SOME TimeOut))``,
+  recInduct bvpSemTheory.evaluate_ind \\ rpt strip_tac \\ fs []
+  THEN1 (* Skip *)
+   (fs [comp_def,bvpSemTheory.evaluate_def,wordSemTheory.evaluate_def]
+    \\ rw [])
+  THEN1 (* Move *) cheat
+  THEN1 (* Assign *) cheat
+  THEN1 (* Tick *)
+   (fs [comp_def,bvpSemTheory.evaluate_def,wordSemTheory.evaluate_def]
+    \\ `t.clock = s.clock` by fs [state_rel_def] \\ fs [] \\ rw []
+    \\ fs [] \\ rw [] \\ rpt (pop_assum mp_tac)
+    \\ fs [state_rel_def,bvpSemTheory.dec_clock_def,wordSemTheory.dec_clock_def])
+  THEN1 (* MakeSpace *) cheat
+  THEN1 (* Raise *) cheat
+  THEN1 (* Return *) cheat
+  THEN1 (* Seq *) cheat
+  THEN1 (* If *) cheat
+  THEN1 (* Call *) cheat);
 
 val _ = export_theory();
